theories/zoo_saturn/inf_queue_mpmc_1__code.v
@@ -1,0 +1,88 @@
+Require Import zoo.prelude.
+Require Import zoo.language.typeclasses.
+Require Import zoo.language.notations.
+Require Import zoo_std.domain.
+Require Import zoo_std.inf_array.
+Require Import zoo_std.int.
+Require Import zoo_std.optional.
+Require Import zoo.options.
+
+Notation "'inf_queue_mpmc_1٠data'" := (
+  in_type "zoo_saturn.inf_queue_mpmc_1.t" 0
+)(in custom zoo_field
+).
+Notation "'inf_queue_mpmc_1٠front'" := (
+  in_type "zoo_saturn.inf_queue_mpmc_1.t" 1
+)(in custom zoo_field
+).
+Notation "'inf_queue_mpmc_1٠back'" := (
+  in_type "zoo_saturn.inf_queue_mpmc_1.t" 2
+)(in custom zoo_field
+).
+
+Definition inf_queue_mpmc_1٠create : val :=
+  𝗳𝘂𝗻 ⎽ ->
+    { inf_array٠create §optional٠Nothing, 0, 0 }.
+
+Definition inf_queue_mpmc_1٠size : val :=
+  𝗿𝗲𝗰 "size" "t" ->
+    𝗹𝗲𝘁 "front" = "t".{inf_queue_mpmc_1٠front} 𝗶𝗻
+    𝗹𝗲𝘁 "proph" = 𝗽𝗿𝗼𝗽𝗵 𝗶𝗻
+    𝗹𝗲𝘁 "back" = "t".{inf_queue_mpmc_1٠back} 𝗶𝗻
+    𝗶𝗳
+      (𝗹𝗲𝘁 "@tmp" = "t".{inf_queue_mpmc_1٠front} 𝗶𝗻
+       𝗿𝗲𝘀𝗼𝗹𝘃𝗲 𝘀𝗸𝗶𝗽 "proph" "@tmp" ⍮
+       "@tmp")
+      ==
+      "front"
+    𝘁𝗵𝗲𝗻 (
+      int٠positive_part ("back" - "front")
+    ) 𝗲𝗹𝘀𝗲 (
+      "size" "t"
+    ).
+
+Definition inf_queue_mpmc_1٠is_empty : val :=
+  𝗳𝘂𝗻 "t" ->
+    inf_queue_mpmc_1٠size "t" == 0.
+
+Definition inf_queue_mpmc_1٠is_empty_weak : val :=
+  𝗳𝘂𝗻 "t" ->
+    𝗹𝗲𝘁 "front" = "t".{inf_queue_mpmc_1٠front} 𝗶𝗻
+    𝗹𝗲𝘁 "back" = "t".{inf_queue_mpmc_1٠back} 𝗶𝗻
+    "back" ≤ "front".
+
+Definition inf_queue_mpmc_1٠push : val :=
+  𝗳𝘂𝗻 "t" "v" ->
+    𝗹𝗲𝘁 "i" = 𝗳𝗮𝗮 "t".[inf_queue_mpmc_1٠back] 1 𝗶𝗻
+    inf_array٠set
+      "t".{inf_queue_mpmc_1٠data}
+      "i"
+      ‘optional٠Something( "v" ).
+
+Definition inf_queue_mpmc_1٠pop₁ : val :=
+  𝗿𝗲𝗰 "pop" "t" "i" ->
+    𝗺𝗮𝘁𝗰𝗵
+      inf_array٠get "t".{inf_queue_mpmc_1٠data} "i"
+    𝘄𝗶𝘁𝗵
+    | optional٠Nothing ->
+        domain٠yield () ⍮
+        "pop" "t" "i"
+    | optional٠Anything ->
+        𝗳𝗮𝗶𝗹
+    | optional٠Something "v" ->
+        inf_array٠set "t".{inf_queue_mpmc_1٠data} "i" §optional٠Anything ⍮
+        "v"
+    𝗲𝗻𝗱.
+
+Definition inf_queue_mpmc_1٠pop : val :=
+  𝗳𝘂𝗻 "t" ->
+    𝗹𝗲𝘁 "i" = 𝗳𝗮𝗮 "t".[inf_queue_mpmc_1٠front] 1 𝗶𝗻
+    inf_queue_mpmc_1٠pop₁ "t" "i".
+
+Definition inf_queue_mpmc_1٠try_pop : val :=
+  𝗳𝘂𝗻 "t" ->
+    𝗶𝗳 inf_queue_mpmc_1٠is_empty_weak "t" 𝘁𝗵𝗲𝗻 (
+      §None
+    ) 𝗲𝗹𝘀𝗲 (
+      ‘Some( inf_queue_mpmc_1٠pop "t" )
+    ).
