theories/zoo_saturn/inf_queue_mpmc_1__opaque.v
@@ -1,0 +1,10 @@
+Require Import zoo_saturn.inf_queue_mpmc_1__code.
+
+#[global] Opaque inf_queue_mpmc_1٠create.
+#[global] Opaque inf_queue_mpmc_1٠size.
+#[global] Opaque inf_queue_mpmc_1٠is_empty.
+#[global] Opaque inf_queue_mpmc_1٠is_empty_weak.
+#[global] Opaque inf_queue_mpmc_1٠push.
+#[global] Opaque inf_queue_mpmc_1٠pop₁.
+#[global] Opaque inf_queue_mpmc_1٠pop.
+#[global] Opaque inf_queue_mpmc_1٠try_pop.
