theories/zoo_saturn/inf_queue_mpmc_1__types.v
@@ -8,14 +8,14 @@ Require Export zoo_std.optional.
 Require Import zoo.options.
 
 Notation "'data'" := (
-  in_type "zoo_saturn.inf_mpmc_queue_1.t" 0
+  in_type "zoo_saturn.inf_queue_mpmc_1.t" 0
 )(in custom zoo_field
 ).
 Notation "'front'" := (
-  in_type "zoo_saturn.inf_mpmc_queue_1.t" 1
+  in_type "zoo_saturn.inf_queue_mpmc_1.t" 1
 )(in custom zoo_field
 ).
 Notation "'back'" := (
-  in_type "zoo_saturn.inf_mpmc_queue_1.t" 2
+  in_type "zoo_saturn.inf_queue_mpmc_1.t" 2
 )(in custom zoo_field
 ).
